src/lowparse/LowParse.Low.Writers.Instances.fst
@@ -1,0 +1,105 @@
+module LowParse.Low.Writers.Instances
+include LowParse.Low.Writers
+include LowParse.Low.Combinators
+include LowParse.Low.Bytes
+
+module HS = FStar.HyperStack
+module B = LowStar.Buffer
+module U32 = FStar.UInt32
+module HST = FStar.HyperStack.ST
+
+inline_for_extraction
+noextract
+let swrite_nondep_then
+  (h0: HS.mem)
+  (sout: slice (srel_of_buffer_srel (B.trivial_preorder _)) (srel_of_buffer_srel (B.trivial_preorder _)))
+  (pout_from0: U32.t)
+  (#k1: parser_kind)
+  (#t1: Type0)
+  (#p1: parser k1 t1)
+  (#s1: serializer p1 { k1.parser_kind_subkind == Some ParserStrong })
+  (w1: swriter s1 h0 0 sout pout_from0)
+  (#k2: parser_kind)
+  (#t2: Type0)
+  (#p2: parser k2 t2)
+  (#s2: serializer p2 { k2.parser_kind_subkind == Some ParserStrong })
+  (#space_beyond: nat)
+  (w2: swriter s2 h0 space_beyond sout pout_from0)
+: Tot (w: swriter (s1 `serialize_nondep_then` s2) h0 space_beyond sout pout_from0 {
+    swvalue w == (swvalue w1, swvalue w2)
+  })
+= SWriter (Ghost.hide (swvalue w1, swvalue w2)) (fun pout_from ->
+    serialized_length_eq (s1 `serialize_nondep_then` s2) (swvalue w1, swvalue w2);
+    serialize_nondep_then_eq s1 s2 (swvalue w1, swvalue w2);
+    serialized_length_eq s1 (swvalue w1);
+    serialized_length_eq s2 (swvalue w2);
+    let pos1 = swrite w1 pout_from in
+    let pos2 = swrite w2 pos1 in
+    let h' = HST.get () in
+    valid_nondep_then h' p1 p2 sout pout_from;
+    pos2
+  )
+
+module U8 = FStar.UInt8
+module FB = FStar.Bytes
+
+inline_for_extraction
+noextract
+let swrite_bounded_vlbytes
+  (h0: HS.mem)
+  (sout: slice (srel_of_buffer_srel (B.trivial_preorder _)) (srel_of_buffer_srel (B.trivial_preorder _)))
+  (pout_from0: U32.t)
+  (min: nat)
+  (max: nat { min <= max /\ max > 0 /\ max < 4294967296 })
+  (len: U32.t { min <= U32.v len /\ U32.v len <= max })
+  (b: B.lbuffer U8.t (U32.v len) {
+    B.live h0 b /\
+    B.loc_disjoint (B.loc_buffer b) (loc_slice_from sout pout_from0)
+  })
+: Tot (w: swriter (serialize_bounded_vlbytes min max) h0 0 sout pout_from0 {
+    swvalue w == FB.hide (B.as_seq h0 b)
+  })
+= SWriter (Ghost.hide (FB.hide (B.as_seq h0 b))) (fun pout_from ->
+    serialized_length_eq (serialize_bounded_vlbytes min max) (FB.hide (B.as_seq h0 b));
+    length_serialize_bounded_vlbytes min max (FB.hide (B.as_seq h0 b));
+    let pout_payload = pout_from `U32.add` U32.uint_to_t (log256' max) in
+    let payload = B.sub sout.base pout_payload len in
+    B.blit b 0ul payload 0ul len;
+    finalize_bounded_vlbytes min max sout pout_from len
+  )
+
+#push-options "--z3rlimit 16"
+
+inline_for_extraction
+noextract
+let swrite_bounded_vlgenbytes
+  (h0: HS.mem)
+  (sout: slice (srel_of_buffer_srel (B.trivial_preorder _)) (srel_of_buffer_srel (B.trivial_preorder _)))
+  (pout_from0: U32.t)
+  (min: nat)
+  (max: nat { min <= max /\ max > 0 /\ max < 4294967296 })
+  (#kk: parser_kind)
+  (#pk: parser kk (bounded_int32 min max))
+  (#sk: serializer pk { kk.parser_kind_subkind == Some ParserStrong })
+  (wk: leaf_writer_strong sk)
+  (len: U32.t { min <= U32.v len /\ U32.v len <= max })
+  (b: B.lbuffer U8.t (U32.v len) {
+    B.live h0 b /\
+    B.loc_disjoint (B.loc_buffer b) (loc_slice_from sout pout_from0)
+  })
+: Tot (w: swriter (serialize_bounded_vlgenbytes min max sk) h0 0 sout pout_from0 {
+    swvalue w == FB.hide (B.as_seq h0 b)
+  })
+= SWriter (Ghost.hide (FB.hide (B.as_seq h0 b))) (fun pout_from ->
+    serialized_length_eq (serialize_bounded_vlgenbytes min max sk) (FB.hide (B.as_seq h0 b));
+    length_serialize_bounded_vlgenbytes min max sk (FB.hide (B.as_seq h0 b));
+    serialized_length_eq sk len;
+    let pout_payload = swrite (swrite_leaf wk h0 sout pout_from0 len) pout_from in
+    let payload = B.sub sout.base pout_payload len in
+    B.blit b 0ul payload 0ul len;
+    let h = HST.get () in
+    valid_bounded_vlgenbytes min max pk sout pout_from h;
+    pout_payload `U32.add` len
+  )
+
+#pop-options
